tests/custard/EraseAbbrev.fst
@@ -1,0 +1,15 @@
+module EraseAbbrev
+open FStar.All
+open FStar.IO
+module G = FStar.Ghost
+
+inline_for_extraction noextract
+let step_t (n:Prims.int) = x:Prims.int -> g:G.erased Prims.int -> y:Prims.int -> Tot Prims.int
+
+let add3 : step_t 0 = fun x g y -> x + y
+let add4 (n:Prims.int) : step_t n = fun x g y -> x + y + n
+
+let main () : ML unit =
+  print_string (string_of_int (add3 3 (G.hide 7) 4));
+  print_string (string_of_int (add4 1 3 (G.hide 7) 4));
+  print_string "\n"
